add proof for Karatsuba's multiplication

specs/experimental/rsapss/Spec.RSA.Bignum.fst
@@ -25,6 +25,131 @@ let mod_inv_u64 n0 =
       (ub, vb)) (u64 1, u64 0) in
   vb
 
+(* Karatsuba's multiplication *)
+type sign =
+  | Positive : sign
+  | Negative : sign
+
+val abs_sub:
+  #aBits:size_pos -> #bBits:size_pos{bBits <= aBits} ->
+  a:bignum aBits -> b:bignum bBits -> Pure (tuple2 sign (bignum aBits))
+  (requires True)
+  (ensures (fun (s, res) -> bn_v res = abs (bn_v a - bn_v b) /\ s = (if bn_v a >= bn_v b then Positive else Negative)))
+let abs_sub #aBits #bBits a b =
+  if (bn_is_less a b)
+  then begin
+    let res = bn_sub b a in
+    pow2_le_compat aBits bBits;
+    let res = bn_cast_gt aBits res in
+    (Negative, res) end
+  else begin
+    assert (bn_v a >= bn_v b);
+    (Positive, bn_sub a b) end
+
+val lemma_add_sign:
+  c0:nat -> c1:nat -> c2:nat ->
+  a0:nat -> a1:nat -> a2:nat ->
+  b0:nat -> b1:nat -> b2:nat ->
+  sa2:sign -> sb2:sign -> Lemma
+  (requires (c0 == a0 * b0 /\ c1 == a1 * b1 /\ c2 == a2 * b2 /\
+             a2 == abs (a0 - a1) /\ b2 == abs (b0 - b1) /\
+	     sa2 = (if (a0 >= a1) then Positive else Negative) /\
+	     sb2 = (if (b0 >= b1) then Positive else Negative)))
+  (ensures (if (sa2 = sb2) then (c0 + c1 - c2 == a1 * b0 + a0 * b1) else (c0 + c1 + c2 == a1 * b0 + a0 * b1)))
+let lemma_add_sign c0 c1 c2 a0 a1 a2 b0 b1 b2 sa2 sb2 = ()
+
+val add_sign:
+  #a0Bits:size_pos{a0Bits+a0Bits+1 < max_size_t} ->
+  #a1Bits:size_pos{a1Bits+a1Bits < max_size_t /\ a1Bits <= a0Bits} ->
+  c0:bignum (a0Bits + a0Bits) -> c1:bignum (a1Bits + a1Bits) -> c2:bignum (a0Bits + a0Bits) ->
+  a0:bignum a0Bits -> a1:bignum a1Bits -> a2:bignum a0Bits ->
+  b0:bignum a0Bits -> b1:bignum a1Bits -> b2:bignum a0Bits ->
+  sa2:sign -> sb2:sign -> Pure (res:bignum (a0Bits + a0Bits + 1))
+  (requires (bn_v c0 == bn_v a0 * bn_v b0 /\ bn_v c1 == bn_v a1 * bn_v b1 /\ bn_v c2 == bn_v a2 * bn_v b2 /\
+             bn_v a2 == abs (bn_v a0 - bn_v a1) /\ bn_v b2 == abs (bn_v b0 - bn_v b1) /\
+	     sa2 = (if (bn_v a0 >= bn_v a1) then Positive else Negative) /\
+	     sb2 = (if (bn_v b0 >= bn_v b1) then Positive else Negative)))
+  (ensures (fun res -> bn_v res == bn_v (bn_add_carry (bn_mul a1 b0) (bn_mul a0 b1))))
+  #reset-options "--z3rlimit 300 --max_fuel 0"
+let add_sign #a0Bits #a1Bits c0 c1 c2 a0 a1 a2 b0 b1 b2 sa2 sb2 =
+  lemma_add_sign (bn_v c0) (bn_v c1) (bn_v c2) (bn_v a0) (bn_v a1) (bn_v a2) (bn_v b0) (bn_v b1) (bn_v b2) sa2 sb2;
+  let c01 = bn_add_carry c0 c1 in
+  assert (bn_v c01 == bn_v c0 + bn_v c1);
+  if (sa2 = sb2)
+  then begin
+    let res = bn_sub c01 c2 in
+    assert (bn_v res == (bn_v c0 + bn_v c1) - bn_v c2);
+    res end
+  else begin
+    assert ((bn_v c0 + bn_v c1) + bn_v c2 == bn_v a0 * bn_v b1 + bn_v a1 * bn_v b0);
+    lemma_add_sign1 a0Bits a1Bits a0 a1 b0 b1;
+    pow2_le_compat (a0Bits+a0Bits+1) (a0Bits+a1Bits+1);
+    assert ((bn_v c0 + bn_v c1) + bn_v c2 < pow2 (a0Bits + a0Bits + 1));
+    let (c, res) = bn_add c01 c2 in
+    assert (bn_v res == (bn_v c0 + bn_v c1) + bn_v c2);
+    res end
+
+val karatsuba_f:
+  #aBits:size_pos{aBits + aBits < max_size_t} -> #a0Bits:size_pos ->
+  #a1Bits:size_pos{a0Bits + a1Bits = aBits /\ a1Bits <= a0Bits} ->
+  c0:bignum (a0Bits + a0Bits) -> c1:bignum (a1Bits + a1Bits) ->
+  tmp:bignum (a0Bits+a0Bits+1){bn_v tmp < pow2 (a0Bits+a1Bits+1)} -> Pure (res:bignum (aBits + aBits))
+  (requires (bn_v c0 + bn_v c1 * pow2 (a0Bits + a0Bits) + bn_v tmp * pow2 a0Bits < pow2 (aBits + aBits)))
+  (ensures (fun res -> bn_v res == bn_v c0 + bn_v c1 * pow2 (a0Bits + a0Bits) + bn_v tmp * pow2 a0Bits))
+let karatsuba_f #aBits #a0Bits #a1Bits c0 c1 tmp =
+  let c = bn_const_0 #(aBits + aBits) in
+  pow2_lt_compat (aBits + aBits) (a0Bits + a0Bits);
+  let (_, res0) = bn_add c c0 in
+  assert (bn_v res0 == bn_v c + bn_v c0);
+  pow2_lt_compat (aBits + aBits) (a1Bits + a1Bits);
+  let (_, res1) = bn_lshift_add c1 (a0Bits + a0Bits) res0 in
+  assert (bn_v res1 == bn_v c0 + bn_v c1 * pow2 (a0Bits + a0Bits));
+  let tmp = bn_cast_le (a0Bits+a1Bits+1) tmp in
+  pow2_lt_compat (aBits + aBits) (a0Bits + a1Bits + 1);
+  let (_, res2) = bn_lshift_add tmp a0Bits res1 in
+  assert (bn_v res2 == bn_v c0 + bn_v c1 * pow2 (a0Bits + a0Bits) + bn_v tmp * pow2 a0Bits);
+  res2
+
+val karatsuba:
+  aBits:size_pos{aBits + aBits < max_size_t} ->
+  a:bignum aBits -> b:bignum aBits-> Tot (res:bignum (aBits + aBits){bn_v res == bn_v a * bn_v b})
+  (decreases aBits)
+  #reset-options "--z3rlimit 150 --max_fuel 2"
+let rec karatsuba aBits a b =
+  if aBits < 10 * 64 then bn_mul a b
+  else begin
+    let len = blocks aBits 64 in
+    let a0Bits = 64 * (blocks len 2) in
+    let a1Bits = aBits - a0Bits in
+    assert (a1Bits <= a0Bits);
+
+    let a0 = bn_get_bits a 0 a0Bits in
+    let a1 = bn_get_bits a a0Bits aBits in
+    lemma_get_bits aBits a0Bits a a0 a1;
+
+    let b0 = bn_get_bits b 0 a0Bits in
+    let b1 = bn_get_bits b a0Bits aBits in
+    lemma_get_bits aBits a0Bits b b0 b1;
+
+    let (sa2, a2) = abs_sub a0 a1 in
+    let (sb2, b2) = abs_sub b0 b1 in
+
+    let c0 = karatsuba a0Bits a0 b0 in
+    assert (bn_v c0 == bn_v a0 * bn_v b0);
+    let c1 = karatsuba a1Bits a1 b1 in
+    assert (bn_v c1 == bn_v a1 * bn_v b1);
+    let c2 = karatsuba a0Bits a2 b2 in
+    assert (bn_v c2 == bn_v a2 * bn_v b2);
+
+    let tmp = add_sign #a0Bits #a1Bits c0 c1 c2 a0 a1 a2 b0 b1 b2 sa2 sb2 in
+    assert (bn_v tmp == bn_v a0 * bn_v b1 + bn_v a1 * bn_v b0);
+    lemma_karatsuba_mult aBits a0Bits a1Bits (bn_v a) (bn_v a0) (bn_v a1) (bn_v b) (bn_v b0) (bn_v b1);
+    lemma_mul_pow2 aBits a b;
+    let res = karatsuba_f #aBits #a0Bits #a1Bits c0 c1 tmp in
+    assert (bn_v res == bn_v a * bn_v b);
+    res
+  end
+
 (* Montgomery's arithmetic *)
 val mont_pred:
   #nBits:size_pos -> #cBits:size_pos ->
@@ -93,7 +218,8 @@ val mul_mod_mont:
   nInv_u64:bignum 64 -> n:bignum nBits{bn_v n > 0} ->
   a:bignum (nBits+1) -> b:bignum (nBits+1) -> Tot (res:bignum (nBits+1){bn_v res % bn_v n == ((bn_v a * bn_v b) / pow2 rBits) % bn_v n})
 let mul_mod_mont nBits rBits nInv_u64 n a b =
-  let c = bn_mul a b in
+  //let c = bn_mul a b in
+  let c = karatsuba (nBits+1) a b in
   assert (bn_v c < pow2 (nBits + nBits + 2));
   mont_reduction rBits nInv_u64 n c
 
