specs/experimental/rsapss/Spec.RSA.Lemmas.fst
@@ -508,3 +508,56 @@ let lemma_exp_blinding n phi_n p q d m r =
   if (m = 0 || m % p = 0 || m % q = 0) then
     lemma_exp_blinding_0 n phi_n p q d m r
   else lemma_exp_blinding_1 n phi_n p q d m r
+
+(* LEMMAS for Karatsuba's multiplication *)
+val abs: x:int -> Tot (y:nat{(x >= 0 ==> y = x) /\ (x < 0 ==> y = -x)})
+let abs x = if x >= 0 then x else -x
+
+val lemma_distributivity_mult:
+  a:nat -> b:nat -> c:nat -> d:nat -> Lemma
+  ((a + b) * (c + d) = a * c + a * d + b * c + b * d)
+let lemma_distributivity_mult a b c d = ()
+
+val lemma_karatsuba_mult:
+  aBits:size_pos -> a0Bits:size_pos -> a1Bits:size_pos{a0Bits + a1Bits == aBits} ->
+  a:nat{a < pow2 aBits} -> a0:nat{a0 < pow2 a0Bits} -> a1:nat{a1 < pow2 a1Bits} ->
+  b:nat{b < pow2 aBits} -> b0:nat{b0 < pow2 a0Bits} -> b1:nat{b1 < pow2 a1Bits} -> Lemma
+  (requires (a == a1 * pow2 a0Bits + a0 /\ b == b1 * pow2 a0Bits + b0))
+  (ensures (a * b == a1 * b1 * pow2 (a0Bits + a0Bits) + (a0 * b1 + a1 * b0) * pow2 a0Bits + a0 * b0))
+  #reset-options "--z3rlimit 50 --max_fuel 0"
+let lemma_karatsuba_mult aBits a0Bits a1Bits a a0 a1 b b0 b1 =
+  assert (a * b == (a1 * pow2 a0Bits + a0) * (b1 * pow2 a0Bits + b0));
+  lemma_distributivity_mult (a1 * pow2 a0Bits) a0 (b1 * pow2 a0Bits) b0;
+  assert (a * b == a0 * b0 + a1 * b1 * pow2 a0Bits * pow2 a0Bits + a0 * b1 * pow2 a0Bits + a1 * b0 * pow2 a0Bits);
+  pow2_plus a0Bits a0Bits
+
+val lemma_mul_pow2:
+  aBits:size_pos -> a:bignum aBits -> b:bignum aBits -> Lemma
+  (bn_v a * bn_v b < pow2 (aBits + aBits))
+let lemma_mul_pow2 aBits a b =
+  assert (bn_v a * bn_v b < pow2 aBits * pow2 aBits);
+  pow2_plus aBits aBits
+
+val lemma_get_bits:
+  aBits:size_pos -> a0Bits:size_pos{a0Bits % 64 == 0 /\ a0Bits < aBits} -> a:bignum aBits ->
+  a0:bignum a0Bits -> a1:bignum (aBits - a0Bits) -> Lemma
+  (requires (bn_v a0 == bn_v (bn_get_bits a 0 a0Bits) /\ bn_v a1 == bn_v (bn_get_bits a a0Bits aBits)))
+  (ensures (bn_v a == bn_v a0 + bn_v a1 * pow2 a0Bits))
+let lemma_get_bits aBits a0Bits a a0 a1 =
+  assert (bn_v a0 == bn_v a % pow2 a0Bits);
+  assert (bn_v a1 == (bn_v a / pow2 a0Bits) % pow2 (aBits - a0Bits));
+  pow2_modulo_division_lemma_1 (bn_v a) a0Bits aBits;
+  assert (bn_v a1 == (bn_v a % pow2 aBits) / pow2 a0Bits);
+  small_modulo_lemma_1 (bn_v a) (pow2 aBits);
+  assert (bn_v a1 == bn_v a / pow2 a0Bits);
+  euclidean_division_definition (bn_v a) (pow2 a0Bits)
+
+val lemma_add_sign1:
+  a0Bits:size_pos -> a1Bits:size_pos{a0Bits + a1Bits + 1 < max_size_t} ->
+  a0:bignum a0Bits -> a1:bignum a1Bits ->
+  b0:bignum a0Bits -> b1:bignum a1Bits -> Lemma
+  (bn_v a1 * bn_v b0 + bn_v a0 * bn_v b1 < pow2 (a0Bits + a1Bits + 1))
+let lemma_add_sign1 a0Bits a1Bits a0 a1 b0 b1 =
+  assert (bn_v a1 * bn_v b0 + bn_v a0 * bn_v b1 < pow2 a1Bits * pow2 a0Bits + pow2 a0Bits * pow2 a1Bits);
+  pow2_plus a1Bits a0Bits;
+  pow2_double_sum (a0Bits + a1Bits)
