specs/experimental/rsapss/Spec.Bignum.Basic.fsti
@@ -34,30 +34,37 @@ val bignum:bits:size_nat -> Type0
 
 val bn_v:#bits:size_nat -> bignum bits -> GTot (r:nat{r < pow2 bits})
 val bn_const_1:#bits:size_pos -> r:bignum bits{bn_v r == 1}
+val bn_const_0:#bits:size_pos -> r:bignum bits{bn_v r == 0}
 
 val bn_cast_le:#n:size_pos -> m:size_pos{m <= n} -> b:bignum n{bn_v b < pow2 m} -> c:bignum m{bn_v c == bn_v b}
-val bn_cast_gt:#n:size_pos -> m:size_pos{m > n} -> b:bignum n{bn_v b < pow2 m} -> c:bignum m{bn_v c == bn_v b}
+val bn_cast_gt:#n:size_pos -> m:size_pos{m >= n} -> b:bignum n{bn_v b < pow2 m} -> c:bignum m{bn_v c == bn_v b}
 
 val bn_add:#n:size_pos -> #m:size_pos{m <= n} -> a:bignum n -> b:bignum m -> Pure (tuple2 carry (bignum n))
   (requires (True))
   (ensures (fun (c, res) -> bn_v res + uint_v c * pow2 n == bn_v a + bn_v b))
 
-val bn_sub:#n:size_pos -> #m:size_pos{m <= n} -> a:bignum n -> b:bignum m {bn_v a >= bn_v b} -> c:bignum n{bn_v c == bn_v a - bn_v b}
+val bn_add_carry:#n:size_pos{n+1 < max_size_t} -> #m:size_pos{m <= n} -> a:bignum n -> b:bignum m -> Tot (res:bignum (n+1){bn_v res == bn_v a + bn_v b})
+
+val bn_sub:#n:size_pos -> #m:size_pos -> a:bignum n -> b:bignum m {bn_v a >= bn_v b} -> c:bignum n{bn_v c == bn_v a - bn_v b}
 
 val bn_mul:#n:size_pos -> #m:size_pos{n + m < max_size_t} -> a:bignum n -> b:bignum m -> c:bignum (n + m){bn_v c == bn_v a * bn_v b}
 
 val bn_get_bit:#n:size_pos -> b:bignum n -> i:size_nat{i < n} -> c:nat{(c == 0 \/ c == 1) /\ c == (bn_v b / pow2 i) % 2}
-val bn_get_bits:#n:size_pos -> b:bignum n -> i:size_nat{i < n /\ i % 64 == 0} -> j:size_pos{i < j /\ j % 64 == 0 /\ j <= n} -> c:bignum (j - i){bn_v c == (bn_v b / pow2 i) % pow2 (j - i)}
+val bn_get_bits:#n:size_pos -> b:bignum n -> i:size_nat{i < n /\ i % 64 == 0} -> j:size_pos{i < j /\ (j % 64 == 0 /\ j <= n) \/ (j = n)} -> c:bignum (j - i){bn_v c == (bn_v b / pow2 i) % pow2 (j - i)}
 val bn_rshift:#n:size_pos -> b:bignum n -> i:size_pos{i < n /\ i % 64 == 0} -> c:bignum (n - i){bn_v c == bn_v b / pow2 i}
 
 val bn_to_u64:b:bignum 64 -> c:uint64{uint_v c == bn_v b}
 val bn_from_u64:c:uint64 -> b:bignum 64{uint_v c == bn_v b}
 
-val bn_is_less:#n:size_pos -> #m:size_pos -> a:bignum n -> b:bignum m -> c:bool{c == true ==> bn_v a < bn_v b}
+val bn_is_less:#n:size_pos -> #m:size_pos -> a:bignum n -> b:bignum m -> c:bool{if (c) then bn_v a < bn_v b else bn_v a >= bn_v b}
 
 val bn_lshift_mul_add:#n:size_pos -> #m:size_pos{n <= m} -> x:bignum n -> i:size_nat{n + 1 + i <= m} -> y:bignum 64 -> z:bignum m -> Pure (tuple2 carry (bignum m))
   (requires (True))
   (ensures (fun (c, res) -> bn_v res + uint_v c * pow2 m == bn_v x * (pow2 i) * bn_v y + bn_v z))
+
+val bn_lshift_add:#n:size_pos -> #m:size_pos{n <= m} -> x:bignum n -> i:size_nat{n + i <= m} -> z:bignum m -> Pure (tuple2 carry (bignum m))
+  (requires (True))
+  (ensures (fun (c, res) -> bn_v res + uint_v c * pow2 m == bn_v x * (pow2 i) + bn_v z))
 
 val bn_from_bytes_be:#bBytes:size_pos{8 * bBytes < max_size_t} -> b:lbytes bBytes -> Tot (n:bignum (8 * bBytes){bn_v n == nat_from_bytes_be b})
 
